test/compute_degree.lean
@@ -71,10 +71,16 @@ example : nat_degree (monomial 5 c * monomial 1 c + monomial 7 d +
   C a * X ^ 0 + C b * X ^ 5 + C c * X ^ 2 + X ^ 10 + C e * X : R[X]) ≤ 10 :=
 by compute_degree_le
 
-/-  fails with error message `should the degree bound be '10'?`
+/-  fails with error message `should the degree be '10'?`
 example : nat_degree (monomial 5 c * monomial 1 c + monomial 7 d +
   C a * X ^ 0 + C b * X ^ 5 + C c * X ^ 2 + X ^ 10 + C e * X : R[X]) = 9 :=
 by compute_degree
+--/
+
+/-  fails with error message `should the degree bound be '10'?`
+example : nat_degree (monomial 5 c * monomial 1 c + monomial 7 d +
+  C a * X ^ 0 + C b * X ^ 5 + C c * X ^ 2 + X ^ 10 + C e * X : R[X]) ≤ 9 :=
+by compute_degree_le
 --/
 
 example : nat_degree (monomial 5 c * monomial 1 c + monomial 7 d +
